Notes on try/catch

sandbox.lean
@@ -71,17 +71,95 @@ inductive NucleotideBase where
 | thymine: NucleotideBase
 
 structure DecodeError where
-  position : Nat
+  pos : Nat
+  char : Char
 
 abbrev Result := Except DecodeError (List NucleotideBase)
 
-def decodeDNA (s : String) : Result := do
+def decodeDNA (dna : String) : Result := do
   let mut bases : List NucleotideBase := []
-  for (c, i) in s.toList.zipIdx do
+  for (c, i) in dna.toList.zipIdx do
     match c with
     | 'A' => bases := bases ++ [.adenine]
     | 'C' => bases := bases ++ [.cytosine]
     | 'G' => bases := bases ++ [.guanine]
     | 'T' => bases := bases ++ [.thymine]
-    | _   => throw { position := i }
+    | _   => throw { pos := i , char := c}
   return bases
+
+def report (dna : String) : String :=
+  match decodeDNA dna with
+  | .ok l => s!"✅ decoded sequence of length {l.length}"
+  | .error e => s!"❌ invalid character '{e.char}' at position {e.pos}"
+
+#eval report "GATTACA"
+-- "✅ decoded sequence of length 7"
+
+#eval report "TARATATA"
+-- "❌ invalid character 'R' at position 2"
+
+-- Simpler test of the try/catch issue
+inductive E where
+| main (n : Nat) : E
+| alt : E
+
+def f (e : E) (h : ∃ (n : Nat), e = .main n) : Nat :=
+  -- I can't extract n from h since I am not in a proof. Joy
+  match e with
+  | .main m => m
+  | .alt =>
+      have absurd : False := by
+        have ⟨_, eq⟩ := h;
+        exfalso -- or nomatch eq
+      nomatch absurd
+
+-- Leans knows in the second clause that h : ∃ n, E.alt = E.main n
+-- let's assume for a moment that I can turn this into an absurd stuff.
+-- How can I say "I don't need to pattern match that clause?".
+-- Ah, ok, I think I know: nomatch k where k : False does work for
+-- example.
+
+-- A general result would be: if an exception-throwing value is a top-level
+-- try catch and I can prove that the alternate clause is ok, then the whole
+-- stuff is also ok.
+
+def reportAux (dna : String) : Except DecodeError String := do
+    try
+      let l <- decodeDNA dna
+      return s!"✅ decoded sequence of length {l.length}"
+    catch e =>
+      return s!"❌ invalid character '{e.char}' at position {e.pos}"
+
+theorem reportAuxCantFail :
+  ∀ (dna : String), (reportAux dna).isOk = true := by
+    intro dna
+    rw [Except.isOk]
+    rw [Except.toBool.eq_def]
+    rw [reportAux]
+    simp
+    -- Argh, need to decompose the match somehow ...
+    /-
+    ⊢ (match
+        tryCatch ((fun a => toString "✅ decoded sequence of length " ++ toString a.length ++ toString "") <$> decodeDNA dna)
+          fun e =>
+          pure
+            (toString "❌ invalid character '" ++ toString e.char ++ toString "' at position " ++ toString e.pos ++
+              toString "") with
+      | Except.ok a => true
+      | Except.error a => false) =
+      true
+    -/
+    simp [tryCatch, tryCatchThe, MonadExceptOf.tryCatch]
+    admit
+
+def report' (dna : String) : String :=
+  let message? := reportAux dna
+  match message? with
+  | .ok message => message
+  | .error _ => panic! "unreachable!"
+
+#eval report' "GATTACA"
+-- "✅ decoded sequence of length 7"
+
+#eval report' "TARATATA"
+-- "❌ invalid character 'R' at position 2"
